commit

AP/AP/FreshA/Fresh.lean
@@ -3,10 +3,254 @@ import AP.AP.FreshA.Nbhd
 namespace AP
 
 def AStrat.Fresh (a : AStrat) (s : State) (fsp : FSP) : Prop :=
-  -- a.WF ∧ s.aForallWinsDisj fsp a ∧ ∀ (d : DStrat), d.WF →
-  -- ∀ s₁ p, (s₁, p) ∈ s.aPtsSimAt ⟨a, d⟩ → p ∉ s.aVisited s₁
-  sorry
+  a.Fresh1 s fsp ∧ ∀ (d : DStrat), d.WF → ∀ s₁ p p',
+  (s₁, p) ∈ s.aPtsSimAt ⟨a, d⟩ → sys.validTr s₁ p' → p' ≠ p → p' ∉ s.aVisited s₁
+
+-- #check 0 #exit
+
+-- def AStrat.Fresh1Aux (a : AStrat) (s : State) (fsp : FSP) : Prop :=
+--   a.WF ∧ s.aPos ∉ fsp.get 0 ∧ ∀ (d : DStrat), d.WF → ∀ n, ∃ s₁ s₂,
+--   sys.simulate (Strat.f ⟨a, d⟩) s (n * 2) = (s₁, 0) ∧ sys.tr s₁ (a.f s₁) = some s₂ ∧
+--   s₂.aHwsDisj (fsp.offset (n * 2 + 1) |>.insertSet 0 (s.aVisited s₁).toSet)
+-- 
+-- def aFresh1Cnd (s : State) (fsp : FSP) (s₂ : State) : Prop :=
+--   s₂.aHwsDisj # fsp.offset (s₂.diff s) |>.insertSet 0 # s.aVisited s₂.prev |>.toSet
+-- 
+-- noncomputable
+-- def aFresh1 (s : State) (fsp : FSP) : AStrat :=
+--   aSeek # aFresh1Cnd s fsp
 
 -- #check 0 #exit
 
 -----
+
+theorem AStrat.Fresh.fresh1 {a : AStrat} {s fsp} (h : a.Fresh s fsp) : a.Fresh1 s fsp := h.1
+theorem AStrat.Fresh.wf {a : AStrat} {s fsp} (h : a.Fresh s fsp) : a.WF := h.fresh1.wf
+
+theorem AStrat.fresh_iff_alt₁ {a : AStrat} {s fsp} : a.Fresh s fsp ↔
+a.Fresh1 s fsp ∧ ∀ (d : DStrat), d.WF → ∀ s₁ p p',
+(s₁, p) ∈ s.aPtsSimAt ⟨a, d⟩ → sys.validTr s₁ p' → p' ∉ s.aVisited s₁ := by
+  rw [Fresh]
+  symm; use by tauto
+  rintro ⟨h₁, h₂⟩
+  use h₁
+  intro d hd s₁ p p' h₃ h₄
+  by_cases h₅ : p' ≠ p; grind
+  push_neg at h₅; symm at h₅; subst h₅
+  clear h₂ h₄
+  rcases h₁ with ⟨ha, h₁, h₂⟩
+  grind
+
+theorem AStrat.fresh_iff_alt₂ {a : AStrat} {s fsp} [hs : sys.WF s] : a.Fresh s fsp ↔
+a.WF ∧ s.aForallWinsDisj fsp a ∧ ∀ (d : DStrat), d.WF → ∀ s₁ p p',
+(s₁, p) ∈ s.aPtsSimAt ⟨a, d⟩ → sys.validTr s₁ p' → p' ∉ s.aVisited s₁ := by
+  rw [fresh_iff_alt₁]
+  constructor
+  · rintro ⟨⟨ha, h₁, h₂⟩, h₃⟩; use ha, h₁
+  rintro ⟨ha, h₁, h₂⟩
+  refine ⟨⟨ha, h₁, ?_⟩, h₂⟩
+  intro d hd s₁ p h₃ h₄
+  contrapose! h₄; clear h₄
+  apply h₂ d hd s₁ p p h₃; clear h₂
+  exact State.validTr_of_mem_aPtsSimAt h₃
+
+-- #check 0 #exit
+
+-- @[simp]
+-- instance {s fsp} : aFresh1 s fsp |>.WF := by
+--   unfold aFresh1; infer_instance
+
+-- theorem AState.aForallWinsDisj_of_fresh1Aux {s fsp} {a : AStrat} [hs : AState s]
+-- (h : a.Fresh1Aux s fsp) : s.aForallWinsDisj fsp a := by
+--   choose ha h₀ h using h
+--   intro d hd n
+--   specialize h d hd
+--   induction n using Nat.mod_2_ind <;> nm n
+--   · cases n; simpa; nm n
+--     specialize h n
+--     simp at h
+--     choose s₁ h₁ s₂ h₂ h₃ using h
+--     have hs₁ := AState.of_simulate_mul_two_eq_full h₁
+--     have hs₂ := DState.of_tr h₂
+--     simp [Nat.add_mul, h₁, h₂]
+--     choose a₁ ha₁ h₃ using h₃
+--     specialize h₃ d hd 1
+--     simp at h₃
+--     choose s₃ h₃ h₄ using h₃
+--     use s₃, h₃
+--     simp [FSP.hasLe, FSP.insertSet] at h₄ ⊢
+--     intro k hk
+--     have h₅ := h₄ 0
+--     specialize h₄ 1
+--     simp at h₄ h₅
+--     choose h₅ h₆ using h₅
+--     rw [Nat.le_add_one_iff] at hk
+--     rcases hk with hk | rfl
+--     · exact h₆ k hk
+--     · exact h₄
+--   · specialize h n
+--     choose s₁ s₂ h₁ h₂ h₃ using h
+--     have hs₁ := AState.of_simulate_mul_two_eq_full h₁
+--     simp [h₁, h₂]
+--     replace h₃ := State.aPos_notMem_of_aHwsDisj h₃
+--     simp at h₃
+--     simp [FSP.hasLe]
+--     exact h₃.2
+
+-- theorem AState.fresh1_of_fresh1Aux {s fsp} {a : AStrat} [hs : AState s]
+-- (h : a.Fresh1Aux s fsp) : a.Fresh1 s fsp := by
+--   have H₀ := h
+--   choose ha h₀ h using h
+--   use ha, aForallWinsDisj_of_fresh1Aux H₀
+--   intro d hd s₁ p h₁
+--   rw [State.mem_aPtsSimAt_iff_simulate_tr] at h₁
+--   choose hs₁ n h₁ s₂ h₂ h₃ using h₁
+--   simp at h₂ h₃; subst h₃
+--   obtain ⟨n, rfl⟩ := Nat.even_iff_exi.mp # even_of_simulate h₁
+--   specialize h d hd n
+--   simp [h₁, h₂] at h
+--   rw [←AState.aPos_eq_of_tr h₂]
+--   choose a₁ ha₁ h using h
+--   specialize h d hd 0
+--   simp at h
+--   exact h.1
+
+-- theorem AState.exi_fresh1_of_aHwsDisj {s fsp} [hs : AState s]
+-- (h : s.aHwsDisj fsp) : ∃ (a : AStrat), a.Fresh1 s fsp := by
+--   use aFresh1 s fsp
+--   apply hs.fresh1_of_fresh1Aux
+--   use inferInstance
+--   use State.aPos_notMem_of_aHwsDisj h
+--   intro d hd n
+--   induction n
+--   · simp
+--     have h₁ := @hs.aSeek_exi_tr_of (P := aFresh1Cnd s fsp)
+--     specialize h₁ _
+--     · clear h₁
+--       unfold aFresh1Cnd
+--       replace h := aHwsDisj_insert_one_aPos h
+--       choose a₁ ha₁ h using h
+--       have h₁ := h d hd 1
+--       simp at h₁
+--       choose s₁ h₁ h₂ using h₁
+--       use a₁.f s, s₁, h₁, a₁, ha₁
+--       simp [State.diff_eq_of_tr h₁, State.prev_eq_of_tr h₁]
+--       intro d₁ hd₁ n
+--       specialize h d₁ hd₁ (n + 1)
+--       simp_rw [sys.simulate_succ_full'] at h
+--       simp [h₁] at h
+--       choose s₂ h h₃ using h
+--       use s₂, h
+--       simp [FSP.hasLe, FSP.insert, FSP.insertSet, FSP.next] at h₃ ⊢
+--       grind
+--     unfold aFresh1
+--     choose s₂ h₁ h₂ using h₁
+--     use s₂, h₁
+--     unfold aFresh1Cnd at h₂
+--     simp [State.diff_eq_of_tr h₁, State.prev_eq_of_tr h₁] at h₂
+--     exact h₂
+--   nm n ih
+--   choose s₁ s₂ h₁ h₂ h₃ using ih
+--   have hs₁ := AState.of_simulate_mul_two_eq' h₁
+--   have hs₂ := DState.of_tr h₂
+--   choose s₃ h₄ using hd.validTr s₂
+--   have hs₃ := AState.of_tr h₄
+--   simp [Nat.add_mul, h₁, h₂, h₄]
+--   have G₁ := sys.reachable_of_simulate_eq h₁
+--   have G₂ := sys.reachable_right G₁ h₂
+--   have G₃ := sys.reachable_right G₂ h₄
+--   have h₅ := @hs₃.aSeek_exi_tr_of (P := aFresh1Cnd s fsp)
+--   specialize h₅ _
+--   · clear h₅
+--     unfold aFresh1Cnd
+--     replace h₃ := DState.aHwsDisj_insert_two_aPos h₃
+--     choose a₁ ha₁ h₃ using h₃
+--     have H₁ := h₃ d hd 2
+--     simp [h₄] at H₁
+--     choose s₄ H₁ H₂ using H₁
+--     use a₁.f s₃, s₄, H₁, a₁, ha₁
+--     rw [State.diff_eq_of_tr H₁ G₃, State.diff_eq_of_tr h₄ G₂, State.diff_eq_of_tr h₂ G₁]
+--     rw [State.diff_eq_of_simulate_full h₁]
+--     rw [State.prev_eq_of_tr H₁, DState.aVisited_eq_of_tr h₄ G₂, AState.aVisited_eq_of_tr h₂ G₁]
+--     intro d₁ hd₁ n₁
+--     specialize h₃ (d₁.set s₂ # d.f s₂) (DStrat.wf_set_of_tr h₄) (n₁ + 2)
+--     simp_rw [sys.simulate_succ_full'] at h₃
+--     simp [h₄, H₁] at h₃
+--     choose s₅ H₃ H₄ using h₃
+--     use s₅
+--     have hs₄ := sys.wf_of_tr H₁
+--     split_ands
+--     · convert H₃ using 1
+--       symm
+--       apply State.simulate_set_d_eq_of_length_hist_lt ⟨_, h₄⟩
+--       rw [length_hist_eq_of_tr H₁, length_hist_eq_of_tr h₄]
+--       omega
+--     simp
+--     rw [←AState.aPos_eq_of_tr h₂]
+--     simp [FSP.hasLe] at H₄ ⊢
+--     simp [Nat.add_assoc]
+--     intro k hk
+--     cases k
+--     rotate_left
+--     · nm k
+--       specialize H₄ (k + 3) (by omega)
+--       simp at H₄ ⊢
+--       ring_nf at H₄ ⊢
+--       exact H₄
+--     simp
+--     split_ands
+--     · specialize H₄ 2 (by omega)
+--       simp at H₄
+--       exact H₄.1
+--     · specialize H₄ 0 (by omega)
+--       simp at H₄
+--       exact H₄.1
+--     · intro k hk
+--       iterate 2 rw [Nat.le_add_one_iff] at hk
+--       rcases hk with ((hr | rfl) | rfl)
+--       · specialize H₄ 0 (by omega)
+--         simp at H₄
+--         exact H₄.2 k hr
+--       · specialize H₄ 1 (by omega)
+--         simp at H₄
+--         exact H₄
+--       · specialize H₄ 2 (by omega)
+--         simp at H₄
+--         exact H₄.2
+--   choose s₄ h₅ h₆ using h₅
+--   use s₄, h₅
+--   unfold aFresh1Cnd at h₆
+--   rw [State.diff_eq_of_tr h₅ G₃, State.diff_eq_of_tr h₄ G₂, State.diff_eq_of_tr h₂ G₁] at h₆
+--   rw [State.diff_eq_of_simulate_full h₁] at h₆
+--   simp [Nat.add_assoc] at h₆ ⊢
+--   have hs₄ := DState.of_tr h₅
+--   rw [State.prev_eq_of_tr h₅] at h₆
+--   exact h₆
+
+-- theorem State.aPtsSimAt_state_eq_of_point_eq_of_fresh1 {s : State} {a : AStrat} {d : DStrat}
+-- {s₁ s₂ p fsp} [hs : sys.WF s] [hd : d.WF] (h : a.Fresh1 s fsp)
+-- (h₁ : (s₁, p) ∈ s.aPtsSimAt ⟨a, d⟩) (h₂ : (s₂, p) ∈ s.aPtsSimAt ⟨a, d⟩) : s₁ = s₂ := by
+--   choose ha h₃ h₄ using h
+--   specialize h₄ d hd
+--   have H₁ := h₄ _ _ h₁
+--   have H₂ := h₄ _ _ h₂
+--   clear h₄
+--   rw [mem_aPtsSimAt_iff_simulate_tr] at h₁ h₂
+--   choose hs₁ n₁ h₁ s₁' h₅ h₆ using h₁
+--   choose hs₂ n₂ h₂ s₂' h₇ h₈ using h₂
+--   simp at h₅ h₆ h₇ h₈
+--   by_cases H₃ : n₁ = n₂
+--   · subst H₃
+--     simp [h₁] at h₂
+--     exact h₂
+--   exfalso
+--   wlog H₄ : n₁ < n₂ with ih
+--   · push_neg at H₄
+--     specialize @ih s a d s₂ s₁ p fsp _ _ ha h₃
+--     grind
+--   clear H₃
+--   apply H₂; clear H₂
+--   rw [mem_aVisited_iff h₂]
+--   right
+--   use n₁, H₄, s₁, hs₁, h₁
+--   simpa
